Messy progress on DeltaCorrectness.

Security/SaberRqDeltaCorrectness.ec
@@ -59,13 +59,39 @@ qed.
 (*  Error                              *)
 (* ----------------------------------- *)
 
+
+instance ring with Rq
+  op rzero = Rq.zeroXnD1
+  op rone  = Rq.oneXnD1
+  op add   = Rq.( + )
+  op opp   = Rq.([-])
+  op mul   = Rq.( * )
+  op expr  = Rq.ComRing.exp
+  op ofint = Rq.ComRing.ofint
+
+  proof oner_neq0 by apply Rq.ComRing.oner_neq0
+  proof addrA     by apply Rq.ComRing.addrA
+  proof addrC     by apply Rq.ComRing.addrC
+  proof addr0     by apply Rq.ComRing.addr0
+  proof addrN     by apply Rq.ComRing.addrN
+  proof mulr1     by apply Rq.ComRing.mulr1
+  proof mulrA     by apply Rq.ComRing.mulrA
+  proof mulrC     by apply Rq.ComRing.mulrC
+  proof mulrDl    by apply Rq.ComRing.mulrDl
+  proof expr0     by apply Rq.ComRing.expr0
+  proof ofint0    by apply Rq.ComRing.ofint0
+  proof ofint1    by apply Rq.ComRing.ofint1
+  proof exprS     by apply Rq.ComRing.exprS
+  proof ofintS    by apply Rq.ComRing.ofintS
+  proof ofintN    by apply Rq.ComRing.ofintN.
+(*
 clone Matrix as Mat_int with
   type R    <- int,
     op size <- n.
 
 type int_vec = Mat_int.vector.
-
-(*---*) import Mat_Rp Mat_Rq Mat_int.
+*)
+(*---*) import Mat_Rp Mat_Rq.
 
 abbrev ( - ) (pv1 pv2 : Rq_vec) = pv1 + (- pv2).
   
@@ -73,9 +99,11 @@ op errorZq (z1 z2 : Zq) : Zq = z1 - z2.
 op errorRq (p1 p2 : Rq) : Rq = p1 - p2.
 op errorRqv (pv1 pv2 : Rq_vec) : Rq_vec = pv1 - pv2.
 
+(*
 op interrorZq (z1 z2 : Zq) : int = `| Zq.asint z1 - Zq.asint z2 |.
 op interrorRq (p1 p2 : Rq) : int_vec = offunv (fun (i : int) => interrorZq p1.[i] p2.[i]).
 op interrorRqv (pv1 pv2 : Rq_vec) : int_vec list = mkseq (fun (i : int) => interrorRq pv1.[i] pv2.[i]) l.
+*)
 
 
 (*
@@ -90,9 +118,16 @@ op error_bq0 (s bq : Rq_vec) (_A : Rq_mat) : Rq_vec = errorRqv bq (_A *^ s).
 op error_bq0' (s' bq' : Rq_vec) (_A : Rq_mat) : Rq_vec = errorRqv bq' ((trmx _A) *^ s').
 op error_cmq0 (cmq v' m_dec: Rq) : Rq = errorRq cmq (v' + m_dec).
 
+(*
 op interror_bq (s bq : Rq_vec) (_A : Rq_mat) : int_vec list = interrorRqv bq (_A *^ s).
 op interror_bq' (s' bq' : Rq_vec) (_A : Rq_mat) : int_vec list = interrorRqv bq' ((trmx _A) *^ s').
 op interror_cmq (cmq v' m_dec: Rq) : int_vec = interrorRq cmq (v' + m_dec).
+*)
+const poly_q4 : Rq =
+  (BigRq.XnD1CA.bigi predT (fun (i : int) => Zq.inzmod (2 ^ (eq - 2)) ** exp Rq.iX i) 0 n).
+const poly_q4t : Rq =
+  (BigRq.XnD1CA.bigi predT (fun (i : int) => Zq.inzmod (2 ^ (eq - et - 2)) ** exp Rq.iX i) 0 n).
+
 
 op error_bq (_A : Rq_mat) (s : Rq_vec) : Rq_vec = 
   errorRqv (scaleRpv2Rqv (scaleRqv2Rpv (_A *^ s + h))) (_A *^ s).
@@ -107,14 +142,28 @@ op v'_expression (_A : Rq_mat) (s s': Rq_vec) : Rq =
   let bq = (_A *^ s) + (error_bq _A s) in
   (dotp bq s') + (upscaleRq h1 (eq - ep)).
 
-(* Add q / 4t to make error centered around zero *)
 op error_cmq (_A : Rq_mat) (s s': Rq_vec) (m : R2) : Rq =
   let v' = v'_expression _A s s' in
   errorRq (scaleR2t2Rq (scaleRq2R2t (v' + (scaleR22Rq m)))) (v' + (scaleR22Rq m)).
 
+(* Add q / 4t to make error centered around zero *)
+op error_cmq_centered (_A : Rq_mat) (s s': Rq_vec) (m : R2) : Rq = 
+  error_cmq _A s s' m + poly_q4t.
+
 op cmq_expression (_A : Rq_mat) (s s': Rq_vec) (m : R2) : Rq =
   let v' = v'_expression _A s s' in
   v' + (scaleR22Rq m) + error_cmq _A s s' m.
+
+op cmq_expression_centered (_A : Rq_mat) (s s': Rq_vec) (m : R2) =
+  let v' = v'_expression _A s s' in
+  v' + (scaleR22Rq m) + error_cmq_centered _A s s' m - poly_q4t.
+
+lemma eq_cmq_cmqcen  (_A : Rq_mat) (s s': Rq_vec) (m : R2) :
+  cmq_expression _A s s' m = cmq_expression_centered _A s s' m.
+proof. 
+rewrite /cmq_expression /cmq_expression_centered /v'_expression /error_cmq_centered /error_cmq /=.
+by ring.
+qed.
 
 op m'_expression_Rq (_A : Rq_mat) (s s': Rq_vec) (m : R2) : Rq =
   let v = v_expression _A s s' in
@@ -124,6 +173,191 @@ op m'_expression_Rq (_A : Rq_mat) (s s': Rq_vec) (m : R2) : Rq =
 op m'_expression (_A : Rq_mat) (s s': Rq_vec) (m : R2) : R2 = scaleRq2R2 (m'_expression_Rq _A s s' m).
 
 pragma Goals:printall.
+
+
+lemma scaleZ22Zq_PN (z : Z2) : scaleZ22Zq z = scaleZ22Zq (- z).
+proof.
+rewrite /scaleZ22Zq /upscale /shl -eq_inzmod !inzmodK; do 3! congr.
+case (asint z = 0) => [-> //| /neq_ltz [lt0_z | gt0_z]]; move: (Z2.rg_asint z); case => ge0_z lt2_z.
++ by rewrite ltzNge in lt0_z.
++ rewrite -lez_add1r -(lez_add2l (-1)) /= in lt2_z; rewrite -lez_add1r /= in gt0_z.
+  by move: (eqz_leq (asint z) 1); rewrite gt0_z lt2_z /= => ->.
+qed.
+
+lemma scaleR22Rq_PN (p : R2) : scaleR22Rq p = scaleR22Rq (- p).
+proof.
+rewrite /scaleR22Rq !BigRq.XnD1CA.big_seq &(BigRq.XnD1CA.eq_bigr) /= => *.
+by rewrite -rcoeffN scaleZ22Zq_PN.
+qed.
+
+lemma scaleZ22Zq_N (z : Z2) : scaleZ22Zq (- z) = - scaleZ22Zq z.
+proof.
+rewrite /scaleZ22Zq /upscale /shl -inzmodN oppE -eq_inzmod /q -modz_pow2_mul; 1: smt(ge3_eq).
+rewrite expr1 modz_mod -{1}(Ring.IntID.expr1 2) modz_pow2_mul; 1: smt(ge3_eq).
+by rewrite mulNr.
+qed.
+
+lemma scaleR22Rq_N (p : R2) : scaleR22Rq (- p) = - scaleR22Rq p.
+proof.
+rewrite /scaleR22Rq Rq.polyXnD1_sumN /= !BigRq.XnD1CA.big_seq &(BigRq.XnD1CA.eq_bigr) /= => *.
+by rewrite -rcoeffN scaleZ22Zq_N scaleN.
+qed.
+
+lemma dotp_prop1 (_A : Rq_mat) (s s' err: Rq_vec) :
+ (dotp (trmx _A *^ s' + err) s) = (dotp (_A *^ s) s' + dotp err s).
+proof. by rewrite dotpDl dotpC mulmxTv -dotp_mulmxv. qed.
+
+lemma dotp_red (_A : Rq_mat) (s s': Rq_vec) (err err': Rq_vec) :
+  (dotp (trmx _A *^ s' + err') s) - (dotp (_A *^ s + err) s')
+  =
+  dotp err' s - dotp err s'.
+proof.
+rewrite dotp_prop1 addrC. rewrite dotpDl.
+pose dass' := dotp (_A *^ s) s'; pose derrs' := dotp err s'; pose derrs := dotp err' s.
+rewrite addrC. 
+rewrite eq_sym addrC. 
+rewrite opprD. rewrite addrA. rewrite eq_sym. rewrite addrC.
+rewrite &(Rq.ComRing.addrI derrs'). rewrite addrA eq_sym addrA. simplify.
+rewrite subrr.
+rewrite 2!add0r.
+rewrite eq_sym -addrA addrC -addrA.
+rewrite &(Rq.ComRing.addrI (-derrs)).
+rewrite addrA.
+rewrite addrC eq_sym addrC subrr addr0.
+rewrite addrC eq_sym subr_eq0 //.
+qed.
+
+(*
+op m'_expression_reduced_Rq (_A : Rq_mat) (s s': Rq_vec) (m : R2) : Rq =
+   scaleR22Rq m + dotp (error_bq' _A s') s - dotp (error_bq _A s) s' 
+   - error_cmq _A s s' m + upscaleRq h2 (eq - ep).
+
+op m'_expression_reduced (_A : Rq_mat) (s s': Rq_vec) (m : R2) : R2 =
+  scaleRq2R2 (
+  dotp (error_bq' _A s') s - dotp (error_bq _A s) s' 
+  - scaleR22Rq m - error_cmq _A s s' m + upscaleRq h2 (eq - ep)).
+*)
+
+op m'_expression_Rq_reduced1 (_A : Rq_mat) (s s': Rq_vec) (m : R2) : Rq =
+   scaleR22Rq m + dotp (error_bq' _A s') s - dotp (error_bq _A s) s' 
+   - error_cmq _A s s' m + upscaleRq h2 (eq - ep).
+
+lemma eq_m'_m'red1_Rq (_A : Rq_mat) (s s': Rq_vec) (m : R2) :
+  m'_expression_Rq _A s s' m =  m'_expression_Rq_reduced1 _A s s' m.
+proof.
+rewrite /m'_expression_Rq /m'_expression_Rq_reduced1 /v_expression /cmq_expression.
+rewrite /v'_expression /=.
+congr.
+rewrite dotp_prop1. 
+rewrite 3!opprD. 
+rewrite addrA. 
+congr.
+rewrite eq_sym.
+rewrite -addrA.
+rewrite addrC.
+rewrite -(dotp_red _A s s' ((error_bq _A s)) ((error_bq' _A s'))).
+rewrite dotp_prop1.
+rewrite {1}scaleR22Rq_PN.
+rewrite scaleR22Rq_N.
+by ring.
+qed.
+
+op m'_expression_Rq_reduced2 (_A : Rq_mat) (s s': Rq_vec) (m : R2) :
+   Rq = scaleR22Rq m + dotp (error_bq' _A s') s - dotp (error_bq _A s)
+   s' - error_cmq_centered _A s s' m + poly_q4.
+
+lemma eq_m'red1_m'red2_Rq (_A : Rq_mat) (s s': Rq_vec) (m : R2) :
+  m'_expression_Rq_reduced1 _A s s' m = m'_expression_Rq_reduced2 _A s s' m.
+proof.
+rewrite /m'_expression_Rq_reduced1 / m'_expression_Rq_reduced2.
+rewrite /error_cmq_centered /error_cmq /=.
+ring.
+rewrite &(Rq.ComRing.addrI poly_q4) addrA addrA Rq.ComRing.subrr -Rq.ComRing.addrA. 
+rewrite Rq.ComRing.add0r. 
+rewrite Rq.ComRing.ofint0 Rq.ComRing.addr0.
+rewrite Rq.ComRing.addrC &(Rq.ComRing.addIr (- poly_q4t)).
+rewrite -Rq.ComRing.addrA.
+rewrite Rq.ComRing.addrC.
+rewrite Rq.ComRing.subrr Rq.ComRing.add0r.
+rewrite /upscaleRq /upscaleZq /upscale /shl.
+rewrite polyXnD1_eqP => i rng_i.
+rewrite rcoeffZ_sum //=.
+rewrite rcoeffZ_sum //=.
+rewrite !inzmodK. 
+rewrite /poly_q4 /poly_q4t. 
+rewrite polyXnD1_sumN /=.
+rewrite -BigRq.XnD1CA.big_split /=.
+have ->:
+(fun (i0 : int) =>
+       ((inzmod (2 ^ (eq - 2)))%Zq ** exp Rq.iX i0 -
+        (inzmod (2 ^ (eq - et - 2)))%Zq ** exp Rq.iX i0))
+=
+(fun (i0 : int) =>
+       ((inzmod (2 ^ (eq - 2)))%Zq -
+        (inzmod (2 ^ (eq - et - 2))))%Zq ** exp Rq.iX i0).
+rewrite fun_ext /( == ) => x.
+rewrite scaleDl.
+by rewrite scaleN.
+rewrite rcoeffZ_sum //=.
+rewrite -eq_inzmod.
+rewrite oppE. rewrite !inzmodK. 
+rewrite modzNm.
+rewrite modzDm.
+rewrite modzMml.
+rewrite mulrBl.
+rewrite -!exprD_nneg; 1, 2, 3, 4: smt(ge2_ep geep1_eq geet2_ep).
+congr. congr. congr. congr.
+ring.
+congr. congr.
+ring.
+qed.
+
+op m'_expression_Rq_fin (_A : Rq_mat) (s s': Rq_vec) (m : R2) : Rq = 
+  scaleR22Rq m + (poly_q4 + dotp (error_bq' _A s') s - dotp (error_bq _A s) s' 
+  - error_cmq_centered _A s s' m).
+
+lemma eq_m'red2_m'fin_Rq (_A : Rq_mat) (s s': Rq_vec) (m : R2) :
+  m'_expression_Rq_reduced2 _A s s' m = m'_expression_Rq_fin _A s s' m.
+proof.
+rewrite /m'_expression_Rq_reduced2 /m'_expression_Rq_fin. 
+by ring.
+qed.
+
+lemma eq_m'_m'fin_Rq  (_A : Rq_mat) (s s': Rq_vec) (m : R2) :
+  m'_expression_Rq _A s s' m = m'_expression_Rq_fin _A s s' m.
+proof.
+by rewrite eq_m'_m'red1_Rq eq_m'red1_m'red2_Rq eq_m'red2_m'fin_Rq.
+qed.
+
+op m'_expression_fin (_A : Rq_mat) (s s': Rq_vec) (m : R2) : R2 = 
+  scaleRq2R2 (m'_expression_Rq_fin _A s s' m).
+
+lemma eq_m'_m'fin (_A : Rq_mat) (s s': Rq_vec) (m : R2) :
+  m'_expression _A s s' m = m'_expression_fin _A s s' m.
+proof.
+by rewrite /m'_expression /m'_expression_fin eq_m'_m'fin_Rq.
+qed.
+
+
+(* Error Game
+
+module Correctness_Error_Game (S : Scheme, A : Adv_Cor) = {
+   proc main() : bool = {
+      var m: plaintext;
+      var m': plaintext option;
+      var c: ciphertext;
+      var pk: pkey;
+      var sk: skey;
+      
+      (pk, sk) <@ S.kg();
+      m <@ A.choose(pk, sk);
+      c <@ S.enc(pk, m);
+      m' <@ S.dec(sk, c);
+
+      return (Some m = m');
+   }
+}.
+*)
 
 lemma errrng_impl_correct_Zq (m : Z2) (err : Zq) :
   0 <= Zq.asint err < q %/ 2 => m = scaleZq2Z2 (scaleZ22Zq m + err).
@@ -163,6 +397,74 @@ lemma correct_errrng_Zq (m : Z2) (err : Zq) :
  0 <= Zq.asint err < q %/ 2 <=> m = scaleZq2Z2 (scaleZ22Zq m + err).
 proof. by split; [apply errrng_impl_correct_Zq | apply correct_impl_errrng_Zq]. qed.
 
+lemma eq_minq4_q34_modq : Zq.inzmod (- q %/ 4) = Zq.inzmod (3 * q %/ 4).
+proof.
+rewrite -eq_inzmod /q {1 3}(_ : 2 ^ eq = 2 ^ (eq - 2) * 4) 1:(_ : 4 = 2 ^ 2) 1:expr2 // 1:-exprD_nneg;
+        1, 2, 3: smt(ge3_eq).
+rewrite mulrA !mulzK //.
+rewrite modNz 1,2:expr_gt0 //.
+rewrite !pmod_small. admit. admit.
+rewrite opprD /= addrA; ring.
+rewrite mulNr (_ : 4 = 2 ^ 2) 1:expr2 // -exprD_nneg; 1, 2: smt(ge3_eq).
+by rewrite addzA (addzC _ (-2)) addzA.
+qed.
+
+lemma correct_errrng_q4_Zq (m : Z2) (err : Zq) :
+  Zq.asint (Zq.inzmod (- q %/ 4)) <= Zq.asint err \/ Zq.asint err < q %/ 4
+  <=> 
+  m = scaleZq2Z2 (scaleZ22Zq m + (Zq.inzmod (q %/ 4) + err)).
+proof.
+rewrite eq_minq4_q34_modq.
+rewrite -correct_errrng_Zq !inzmodK. 
+split. admit. 
+(*1: case => [geq34_err ltq4_err].
++ have rng_errq4 : 0 <= q %/ 4 %% q + Zq.asint err < q %/ 2.
+  - rewrite pmod_small.
+    * by rewrite (_ : 4 = 2 ^ 2) 1:expr2 /q // divz_ge0 expr2 
+                 2:expr_ge0 3:ltz_divLR 4:ltr_pmulr 4:expr_gt0.
+    rewrite pmod_small in ltq4_err.
+    * by rewrite /q lez_divRL 2:ltz_divLR //= expr_ge0 2:ltr_pmulr 2:expr_gt0.
+    split => [|?].
+    * by rewrite addr_ge0 1:divz_ge0 2:expr_ge0 3:Zq.ge0_asint.
+    * rewrite (ltr_le_trans (q %/ 4 + q %/ 4)) 1:ltr_add2l // lez_eqVlt; left.
+      rewrite /q -divzDl (_ : 4 = 2 ^ 2) 1,3,4:expr2 // 1:dvdz_exp2l; 1: smt(ge3_eq).
+      rewrite eq_sym eqz_div // 1:-expr2 -mulr2z intmulz 1:-{4}expr1 1:-exprD_nneg 3:dvdz_exp2l;
+              1, 2, 3: smt(ge3_eq).
+    by rewrite mulrA divzK 1:-{1}expr1 1:dvdz_exp2l; smt(ge3_eq).
+  split => [|?].
+  - by rewrite modz_ge0 neq_ltz /q; right; apply expr_gt0.
+  - rewrite pmod_small; first move: rng_errq4; case => -> ltq2_errq4 /=.
+    * rewrite (ltr_trans (q %/2)) // ltz_divLR //#.
+    by move: rng_errq4; case => ? ->.
+*)
+admit.
+(*
+case => ?. apply contraLR.
+rewrite !andabP negb_or !negb_and Zq.gtp_asint Zq.ge0_asint /= lezNgt /= -!lezNgt.
+case => ltq34_err geq4_err.
+rewrite (pmod_small (q %/ 4)). admit.
+rewrite pmod_small.
+rewrite addr_ge0 2:ge0_asint 1:divz_ge0 2:expr_ge0 //=.
+rewrite pmod_small in ltq34_err. admit.
+rewrite (ltr_le_trans (q %/ 4 + 3 * q %/ 4)).
+rewrite ltr_add2l //.
+rewrite -divzDl. admit.
+rewrite lez_divLR //.
+rewrite mulrC -intmulz.
+rewrite -mulrS //= intmulz.
+rewrite dvdz_mull.
+rewrite dvdzz.
+rewrite mulrC -intmulz.
+rewrite -mulrS //= intmulz.
+rewrite lezz.
+rewrite (_ : q %/ 2 = q %/ 4 + q %/ 4).
+rewrite -mulr2z intmulz.
+rewrite -eqz_mul // /q 1:-{1}expr1 1:dvdz_exp2l; 1:smt(ge3_eq).
+rewrite mulzA /= eq_sym -dvdz_eq (_ : 4 = 2 ^ 2) 1:expr2 // dvdz_exp2l; 1:smt(ge3_eq).
+rewrite lez_add2l //.
+*)
+qed.
+
 lemma correct_errrng_Rq (m : R2) (err : Rq) :
  (forall (i : int), 0 <= i < n => 0 <= Zq.asint err.[i] < q %/ 2)
  <=> 
@@ -174,59 +476,30 @@ split; rewrite polyXnD1_eqP => [coeff_errrng i rng_i | corr i rng_i]; 2: move: (
 + by apply correct_impl_errrng_Zq.
 qed.
 
-lemma test0 (_A : Rq_mat) (s s' err: Rq_vec) :
- (dotp (trmx _A *^ s' + err) s) = (dotp (_A *^ s) s' + dotp err s).
-proof. by rewrite dotpDl dotpC mulmxTv -dotp_mulmxv. qed.
-
-lemma test1 (_A : Rq_mat) (s s': Rq_vec) (err err': Rq_vec) :
-  (dotp (trmx _A *^ s' + err') s) - (dotp (_A *^ s + err) s')
-  =
-  dotp err' s - dotp err s'.
+lemma correct_errrng_q4_Rq (m : R2) (err : Rq) :
+ (forall (i : int), 0 <= i < n => 
+  Zq.asint (Zq.inzmod (- q %/ 4)) <= Zq.asint err.[i] \/ Zq.asint err.[i] < q %/ 4)
+ <=> 
+ (m = scaleRq2R2 (scaleR22Rq m + 
+                 ((BigRq.XnD1CA.bigi predT (fun (i : int) => Zq.inzmod (q %/ 4) ** exp Rq.iX i) 0 n) +
+                   err))).
 proof.
-rewrite test0 addrC. rewrite dotpDl.
-pose dass' := dotp (_A *^ s) s'; pose derrs' := dotp err s'; pose derrs := dotp err' s.
-rewrite addrC. 
-rewrite eq_sym addrC. 
-rewrite opprD. rewrite addrA. rewrite eq_sym. rewrite addrC.
-rewrite &(Rq.ComRing.addrI derrs'). rewrite addrA eq_sym addrA. simplify.
-rewrite subrr.
-rewrite 2!add0r.
-rewrite eq_sym -addrA addrC -addrA.
-rewrite &(Rq.ComRing.addrI (-derrs)).
-rewrite addrA.
-rewrite addrC eq_sym addrC subrr addr0.
-rewrite addrC eq_sym subr_eq0 //.
+split; rewrite polyXnD1_eqP => [coeff_errrng i rng_i | corr i rng_i]; 2: move: (corr i rng_i);
+       rewrite rcoeffZ_sum //= 2!rcoeffD rcoeffZ_sum //= rcoeffZ_sum //=;
+       rewrite -/(Zq.Sub.insubd (q %/ 4 %% q)) -/(Zq.inzmod (q %/ 4)).
++ by apply /correct_errrng_q4_Zq /(coeff_errrng i rng_i).
++ by rewrite (correct_errrng_q4_Zq m.[i] err.[i]).
 qed.
+
+
+op m'_expression_reduced_Rq (_A : Rq_mat) (s s': Rq_vec) (m : R2) : Rq =
+   scaleR22Rq m + dotp (error_bq' _A s') s - dotp (error_bq _A s) s' 
+   - error_cmq _A s s' m + upscaleRq h2 (eq - ep).
 
 op m'_expression_reduced (_A : Rq_mat) (s s': Rq_vec) (m : R2) : R2 =
   scaleRq2R2 (
   dotp (error_bq' _A s') s - dotp (error_bq _A s) s' 
   - scaleR22Rq m - error_cmq _A s s' m + upscaleRq h2 (eq - ep)).
-
-instance ring with Rq
-  op rzero = Rq.zeroXnD1
-  op rone  = Rq.oneXnD1
-  op add   = Rq.( + )
-  op opp   = Rq.([-])
-  op mul   = Rq.( * )
-  op expr  = Rq.ComRing.exp
-  op ofint = Rq.ComRing.ofint
-
-  proof oner_neq0 by apply Rq.ComRing.oner_neq0
-  proof addrA     by apply Rq.ComRing.addrA
-  proof addrC     by apply Rq.ComRing.addrC
-  proof addr0     by apply Rq.ComRing.addr0
-  proof addrN     by apply Rq.ComRing.addrN
-  proof mulr1     by apply Rq.ComRing.mulr1
-  proof mulrA     by apply Rq.ComRing.mulrA
-  proof mulrC     by apply Rq.ComRing.mulrC
-  proof mulrDl    by apply Rq.ComRing.mulrDl
-  proof expr0     by apply Rq.ComRing.expr0
-  proof ofint0    by apply Rq.ComRing.ofint0
-  proof ofint1    by apply Rq.ComRing.ofint1
-  proof exprS     by apply Rq.ComRing.exprS
-  proof ofintS    by apply Rq.ComRing.ofintS
-  proof ofintN    by apply Rq.ComRing.ofintN.
 
 lemma test (_A : Rq_mat) (s s': Rq_vec) (m : R2) :
   m'_expression _A s s' m = m'_expression_reduced _A s s' m.
@@ -237,37 +510,27 @@ congr.
 congr.
 ring.
 rewrite addrC.
-rewrite test0.
+rewrite dotp_prop1.
 ring.
 rewrite dotpDl. ring.
 qed.
 
-lemma scaleZ22Zq_PN (z : Z2) : scaleZ22Zq z = scaleZ22Zq (- z).
+lemma eq_m'exp_Rq  (_A : Rq_mat) (s s': Rq_vec) (m : R2) :
+  m'_expression_Rq _A s s' m = m'_expression_reduced_Rq _A s s' m.
 proof.
-rewrite /scaleZ22Zq /upscale /shl -eq_inzmod !inzmodK; do 3! congr.
-case (asint z = 0) => [-> //| /neq_ltz [lt0_z | gt0_z]]; move: (Z2.rg_asint z); case => ge0_z lt2_z.
-+ by rewrite ltzNge in lt0_z.
-+ rewrite -lez_add1r -(lez_add2l (-1)) /= in lt2_z; rewrite -lez_add1r /= in gt0_z.
-  by move: (eqz_leq (asint z) 1); rewrite gt0_z lt2_z /= => ->.
-qed.
-
-lemma scaleR22Rq_PN (p : R2) : scaleR22Rq p = scaleR22Rq (- p).
-proof.
-rewrite /scaleR22Rq !BigRq.XnD1CA.big_seq &(BigRq.XnD1CA.eq_bigr) /= => *.
-by rewrite -rcoeffN scaleZ22Zq_PN.
-qed.
-
-lemma scaleZ22Zq_N (z : Z2) : scaleZ22Zq (- z) = - scaleZ22Zq z.
-proof.
-rewrite /scaleZ22Zq /upscale /shl -inzmodN oppE -eq_inzmod /q -modz_pow2_mul; 1: smt(ge3_eq).
-rewrite expr1 modz_mod -{1}(Ring.IntID.expr1 2) modz_pow2_mul; 1: smt(ge3_eq).
-by rewrite mulNr.
-qed.
-
-lemma scaleR22Rq_N (p : R2) : scaleR22Rq (- p) = - scaleR22Rq p.
-proof.
-rewrite /scaleR22Rq Rq.polyXnD1_sumN /= !BigRq.XnD1CA.big_seq &(BigRq.XnD1CA.eq_bigr) /= => *.
-by rewrite -rcoeffN scaleZ22Zq_N scaleN.
+rewrite /m'_expression_Rq /m'_expression_reduced_Rq /v_expression /cmq_expression.
+rewrite /v'_expression /=.
+congr.
+rewrite dotp_prop1. rewrite 3!opprD. rewrite addrA. 
+congr.
+rewrite eq_sym.
+rewrite -addrA.
+rewrite addrC.
+rewrite -(dotp_red _A s s' ((error_bq _A s)) ((error_bq' _A s'))).
+rewrite dotp_prop1.
+rewrite {1}scaleR22Rq_PN.
+rewrite scaleR22Rq_N.
+by ring.
 qed.
 
 (*
